hash bnodes per split with holes+

src/IsoCan.v
@@ -1,10 +1,12 @@
-From mathcomp Require Import all_ssreflect.
+From mathcomp Require Import all_ssreflect fingraph.
 Set Implicit Arguments.
 Unset Strict Implicit.
 Unset Printing Implicit Defensive.
 From RDF Require Export Rdf Triple Term.
 
 Section IsoCan.
+  Axiom todo: forall t,t.
+
   Variable I B L: countType.
 
   (*   Definition isocanonical_function (M : B -> B) (g : rdf_graph_) :=
@@ -20,9 +22,9 @@ Section IsoCan.
     Section Hash.
 
       Record hash (T : Type) := mkHinput {
-                                      input : T ;
-                                      current_hash : h
-                                    }.
+                                   input : T ;
+                                   current_hash : h
+                                 }.
 
       Lemma by_perf_hash (i : @term I B L) (o : h) (eqb : hashTerm i == o) : hashTerm i = o.
       Proof. apply /eqP. apply eqb. Qed.
@@ -55,13 +57,11 @@ Section IsoCan.
         Canonical hin_ct := Eval hnf in CountType (hash T) hin_canCountMixin.
         Definition hin_canPOrderMixin := PcanPOrderMixin (@pickleK hin_ct).
         Canonical hin_POrderType := Eval hnf in POrderType tt (hash T) hin_canPOrderMixin.
+
       End CountHash.
-
-      (* Definition hash := hi_term. *)
     End Hash.
-    Definition hash_term := @term I (hash B) L.
 
-    (* Let is_bnode := (@is_bnode I (hash B) L). *)
+    Definition hash_term := @term I (hash B) L.
 
     Definition eqb_t_hi (t : @term I B L) (ht : hash_term) : bool :=
       match t, ht with
@@ -79,8 +79,8 @@ Section IsoCan.
       else if eqb_t_hi t p then Some p
            else if eqb_t_hi t o then Some o
                 else None.
-    
-    Definition is_some {T : Type} (ot : option T) : bool := 
+
+    Definition is_some {T : Type} (ot : option T) : bool :=
       match ot with Some _ => true | None => false end.
 
     Definition hash_graph := @rdf_graph I (hash B) L.
@@ -89,27 +89,13 @@ Section IsoCan.
       let otrs := (map (get_triple t) (graph g)) in
       head None (filter is_some otrs).
 
-    (*     Definition lookup_hash (g : rdf_graph I (hash B) L) (b : term I B L): option (hash B) :=
-      let ot := get b g in
-      match ot with 
-      | Some (Bnode hin) => Some hin
-      | _ => None
-      end. *)
-
     Definition lookup_hash (b : hash_term): option (hash B) :=
-      match b with 
+      match b with
       | Bnode hin => Some hin
       | _ => None
       end.
 
-
     Section Partition.
-
-      (*     Definition eq_rel (g : rdf_graph I (hash B) L) (b1 b2 : term I B L ) : bool :=
-      match (lookup_hash b1), (lookup_hash b2) with
-      | Some hin1, Some hin2 => current_hash hin1 == current_hash hin2
-      | _,_ => false
-      end. *)
 
       Definition eq_rel (b1 b2 : hash_term) : bool :=
         match (lookup_hash b1), (lookup_hash b2) with
@@ -135,9 +121,10 @@ Section IsoCan.
         end.
 
       Definition mkPartition (g : hash_graph) : partition :=
-        let bns := (bnodes g) in
+        let bnodes := (bnodes g) in
         let equiv := (fun b => (fun t=> eq_rel b t)) in
-        let P := undup (map (fun b=> (partitionate (equiv b) bns).1 ) bns) in
+        (* undup up to permutation *)
+        let P := undup (map (fun b=> (partitionate (equiv b) bnodes).1 ) bnodes) in
         let ohs := map (fun bs => map lookup_hash bs) P in
         map unwrap ohs.
 
@@ -146,7 +133,7 @@ Section IsoCan.
                              g : hash_graph ;
                              p_wf : P == mkPartition g  ;
                              has_b : all (fun p=> ~~ (nilp p)) P ;
-                             diff_hashes : uniq P 
+                             diff_hashes : uniq P
 
                            }.
 
@@ -198,9 +185,7 @@ Section IsoCan.
       Definition is_intermediate (p : partition) :=
         ~~ is_fine p && ~~ is_coarse p.
 
-    End Partition. 
-
-
+    End Partition.
 
     Definition init_bnode (b : B) : (hash B) :=
       mkHinput b h0.
@@ -208,11 +193,14 @@ Section IsoCan.
     Definition init_hash (g : rdf_graph) : hash_graph :=
       relabeling init_bnode g.
 
+    (* assumes order in the part *)
     Definition cmp_part (p1 p2 : part) : bool :=
       all2 (fun b1 b2 => input b1 == input b2) p1 p2.
 
-    Definition partition_didnt_change (g h: hash_graph) : bool :=
-      let pg := mkPartition g in 
+    (* assumes order in partition *)
+    (* answers true if every part in the partition of g is equal to the respective part in h *)
+    Definition cmp_partition (g h: hash_graph) : bool :=
+      let pg := mkPartition g in
       let ph := mkPartition h in
       all2 (fun p1 p2 => cmp_part p1 p2) pg ph.
 
@@ -223,31 +211,45 @@ Section IsoCan.
       | O => g
       | S n' =>
           let h := update_bnodes g in
-          if partition_didnt_change g h then h else
+          if cmp_partition g h || is_fine (mkPartition h) then h else
             iterate h n'
       end.
-
+    
     Definition hashNodes (g : rdf_graph) : hash_graph :=
       let ini := init_hash g in
       iterate ini (size (graph g)).
-    
 
+    Definition hashNodes_initialized (g : hash_graph) : hash_graph :=
+      iterate g (size (graph g)).
 
-    (*   Definition cmp_bnode (b : B) (t : hash_term) : bool :=
-    match t with
-    | Bnode hin => b == hin
-    | _ => false
-    end. *)
+    Definition reachability_rel (g : hash_graph) (t1 t2 : hash_triple) : bool :=
+      todo _.
+
+    Definition blank_node_split (t u v : Type) (g : @rdf_graph t u v) : seq (@rdf_graph t u v) :=
+      todo _.
+
+    Definition ground_split {t u v : Type} (g : @rdf_graph t u v) : @rdf_graph t u v :=
+      todo _.
+
+    Lemma merge_split {t u v : Type} (g : @rdf_graph t u v) :
+      merge_rdf_graph (merge_seq_rdf_graph (blank_node_split g)) (ground_split g) = g. Admitted.
+
+    Definition hashBnodesPerSplit (g : hash_graph) : hash_graph :=
+      let splitG := blank_node_split g in
+      foldr (@merge_rdf_graph I (hash B) L) (@empty_rdf_graph I (hash B) L) splitG.
+
+    Definition cmp_bnode (b : B) (t : hash_term) : bool :=
+      match t with
+      | Bnode hin => b == (input hin)
+      | _ => false
+      end.
+
     Definition lookup_bnode_in_triple (t : hash_triple) (b : B) : hash_term :=
-      let (s,p,o,_,_,_) := t in 
-      let is_b := (fun t : hash_term => match t with
-                                     | Bnode hin => b == (input hin)
-                                     | _ => false
-                                     end) in
-      if is_b s then s 
-      else if is_b p then p
+      let (s,p,o,_,_,_) := t in
+      if cmp_bnode b s then s
+      else if cmp_bnode b p then p
            else o.
-    
+
     (* Definition lookup_bnode (b : B) (g : hash_graph) : option h := *)
     (*   filter (fun t => match t with *)
     (*                    | Bnode hin => b == hin *)
@@ -255,10 +257,10 @@ Section IsoCan.
     (*                    end) (graph g). *)
 
     (* Lemma hash_dont_get_equal (g : hash_graph) (b1 b2: B) : True. *)
-    
-    
+
+
     (* { hash_term | is_true is_bnode }) : forall n, n+1. *)
-    
+
     (* () *)
     (*     forall (g : rdf_graph) (hms : seq hashmap) *)
     (*            (ghashh : hashNodes g = hms) *)
@@ -268,7 +270,7 @@ Section IsoCan.
     (*       (lookup_hashmap (nth [::] hms i) x != lookup_hashmap (nth [::] hms i) y) *)
     (*       -> lookup_hashmap (nth [::] hms j) x != lookup_hashmap (nth [::] hms j) y. *)
 
-    (* 
+    (*
     Hypothesis hashNodes_preserves_isomorphism :
       forall (g h: rdf_graph) (isogh : iso g h)
              (hash_g hash_h: hashmap)
@@ -277,14 +279,14 @@ Section IsoCan.
              (b : term) (bing : b \in (bnodes (g)))
              (c : term) (cinh : c \in (bnodes (h))),
       exists μ, (relabeling_term μ b) = c -> lookup_hashmap hash_g b = lookup_hashmap hash_h c. *)
-    
+
     (* Hypothesis perfectHashingSchemeTriple : injective hashTriple. *)
 
     Variable hashBag : (seq (hash B) -> (hash B)).
-    Hypothesis hashBag_assoc : forall (l l1 l2 l3: seq (hash B)) (perm : l = l1 ++ l2 ++ l3),
+    Hypothesis hashBag_assoc : forall (l1 l2 l3: seq (hash B)),
         hashBag ([:: hashBag (l1 ++ l2)] ++ l3) = hashBag (l1 ++ [:: hashBag (l2 ++ l3)]).
-    Hypothesis hashBag_comm : forall (l l1 l2: seq (hash B)) (perm : l = l1 ++ l2),
-        hashBag l = hashBag (l2 ++ l1).
+    Hypothesis hashBag_comm : forall (l1 l2: seq (hash B)),
+        hashBag (l1 ++ l2) = hashBag (l2 ++ l1).
 
   End IsoCanAlgorithm.
   (* Hypothesis rdf_total_order   *)
